coq/ZF/Meta/Test/Set/Pair.v
@@ -1,0 +1,115 @@
+Require Import Coq.Lists.List.
+Require Import Coq.Strings.String.
+
+Require Import ZF.Meta.Ctx.
+Require Import ZF.Meta.Env.
+Require Import ZF.Meta.HasTy.
+Require Import ZF.Meta.HasTyIn.
+Require Import ZF.Meta.Term.
+Require Import ZF.Meta.Ty.
+
+Require Import ZF.Meta.Test.Decl.Class.Equiv.
+Require Import ZF.Meta.Test.Decl.Class.Incl.
+Require Import ZF.Meta.Test.Decl.Set.Pair.
+
+Import ListNotations.
+
+(* Environment.                                                                 *)
+
+Definition env : Env := Env.unions
+  [ Pair.env
+  ; Incl.env
+  ; Equiv.env
+  ].
+
+(* Propositions.                                                                *)
+
+(* Proposition Charac : forall a b, forall x, x :< pair a b <-> x = a \/ x = b. *)
+Definition Charac : Term :=
+  All VarTySet
+    (All VarTySet
+      (All VarTySet
+        (Iff
+          (Elem (Var 0) (Ident "pair" [Var 2; Var 1]))
+          (Or
+            (Equal (Var 0) (Var 2))
+            (Equal (Var 0) (Var 1)))))).
+
+(* Proposition IsInL : forall a b, a :< pair a b.                               *)
+Definition IsInL : Term :=
+  All VarTySet
+    (All VarTySet
+      (Elem (Var 1) (Ident "pair" [Var 1; Var 0]))).
+
+(* Proposition IsInR : forall a b, b :< pair a b.                               *)
+Definition IsInR : Term :=
+  All VarTySet
+    (All VarTySet
+      (Elem (Var 0) (Ident "pair" [Var 1; Var 0]))).
+
+(* Proposition ToClassIncl : forall A a b,                                      *)
+(* A a /\ A b <-> Incl (toClass (pair a b)) A.                                  *)
+Definition ToClassIncl : Term :=
+  All VarTyClass
+    (All VarTySet
+      (All VarTySet
+        (Iff
+          (And
+            (App (Var 2) (Var 1))
+            (App (Var 2) (Var 0)))
+          (Ident "Incl"
+            [Ident "toClass" [Ident "pair" [Var 1; Var 0]]; Var 2])))).
+
+(* Proposition typing.                                                          *)
+
+(* The characterization of membership in a pair is well sorted.                 *)
+Proposition CharacCheck : HasTyIn env Ctx.empty Charac TyProp.
+Proof.
+  (* Proof by Hermes + gpt 5.5                                                  *)
+  apply HasTyAll, HasTyAll, HasTyAll, HasTyIff.
+  - apply HasTyElem.
+    + apply (HasTyVar _ _ _ TySet). reflexivity.
+    + apply pairCheckIdent; reflexivity.
+  - apply HasTyOr; apply HasTyEqual; apply (HasTyVar _ _ _ TySet); reflexivity.
+Qed.
+
+(* The left element belongs to its pair, and it is well sorted.                 *)
+Proposition IsInLCheck : HasTyIn env Ctx.empty IsInL TyProp.
+Proof.
+  (* Proof by Hermes + gpt 5.5                                                  *)
+  apply HasTyAll, HasTyAll, HasTyElem.
+  - apply (HasTyVar _ _ _ TySet). reflexivity.
+  - apply pairCheckIdent; reflexivity.
+Qed.
+
+(* The right element belongs to its pair, and it is well sorted.                *)
+Proposition IsInRCheck : HasTyIn env Ctx.empty IsInR TyProp.
+Proof.
+  (* Proof by Hermes + gpt 5.5                                                  *)
+  apply HasTyAll, HasTyAll, HasTyElem.
+  - apply (HasTyVar _ _ _ TySet). reflexivity.
+  - apply pairCheckIdent; reflexivity.
+Qed.
+
+(* Containment of both elements and class inclusion are well sorted.            *)
+Proposition ToClassInclCheck : HasTyIn env Ctx.empty ToClassIncl TyProp.
+Proof.
+  (* Proof by Hermes + gpt 5.5                                                  *)
+  apply HasTyAll, HasTyAll, HasTyAll, HasTyIff.
+  - apply HasTyAnd.
+    + apply HasTyApp.
+      * apply (HasTyVar _ _ _ TyClass). reflexivity.
+      * apply (HasTyVar _ _ _ TySet). reflexivity.
+    + apply HasTyApp.
+      * apply (HasTyVar _ _ _ TyClass). reflexivity.
+      * apply (HasTyVar _ _ _ TySet). reflexivity.
+  - apply HasTyIdent with (argTys := [TyClass; TyClass]). 1: reflexivity.
+    apply HasTysCons.
+    + apply HasTyIdent with (argTys := [TySet]). 1: reflexivity.
+      apply HasTysCons.
+      * apply pairCheckIdent; reflexivity.
+      * apply HasTysNil.
+    + apply HasTysCons.
+      * apply (HasTyVar _ _ _ TyClass). reflexivity.
+      * apply HasTysNil.
+Qed.
